improve handling of statics

case_studies/tests/src/statics.rs
@@ -1,42 +1,43 @@
+#![allow(unused)]
 
 #[rr::name("MYINT")]
 static MYINT: i32 = 42;
 
-#[rr::requires(#iris "initialized π \"MYINT\" 42")]
+#[rr::requires("static_has_refinement \"MYINT\" 42")]
 #[rr::returns("42")]
 fn read_static_1() -> i32 {
     MYINT
 }
 
 #[rr::params("x")]
-#[rr::requires(#iris "initialized π \"MYINT\" x")]
+#[rr::requires("static_has_refinement \"MYINT\" x")]
 #[rr::returns("x")]
 fn ref_static_1() -> &'static i32 {
     &MYINT
 }
 
-#[rr::requires(#iris "initialized π \"MYINT\" 42")]
-#[rr::returns("()")]
+#[rr::requires("static_has_refinement \"MYINT\" 42")]
 fn read_static_2() {
     let r = ref_static_1();
     let _ = *r;
 }
 
-// TODO
-#[rr::skip]
 #[rr::params("x")]
-#[rr::requires(#iris "initialized π \"MYINT\" x")]
+#[rr::requires("static_has_refinement \"MYINT\" x")]
 #[rr::returns("Some x")]
 fn ref_static_2() -> Option<&'static i32> {
     Some(&MYINT)
 }
 
-// TODO: need to properly put lifetimes instead of placeholder_lft
-#[rr::skip]
-#[rr::requires(#iris "initialized π \"MYINT\" 42")]
-#[rr::returns("()")]
+#[rr::requires("static_has_refinement \"MYINT\" 42")]
 fn read_static_3() {
     let r = ref_static_2();
     let r2 = r.unwrap();
     let _ = *r2;
+}
+
+#[rr::requires("static_has_refinement \"MYINT\" 42")]
+#[rr::returns("*[ 42; 42 ]")]
+fn read_static_4() -> (i32, i32) {
+    (MYINT, MYINT)
 }
